Strata/Languages/Boogie/OldExpressions.lean
@@ -392,6 +392,7 @@ theorem IsOldPredNormalize :
       case neg Hneg' =>
         unfold BoogieIdent.unres at *
         unfold normalizeOldExpr at Hold
+        unfold BoogieIdent.unres at *
         split at Hold <;> simp_all
         split at Hold <;> simp_all
         unfold normalizeOldExpr at Hold
